$\Large{2.32 \\ \text{(a) } x \in \Bbb{R} \backslash \{7 \}. \\ \text{(b) } x \in \Bbb{R}. \\ \text{(c) } x \in \Bbb{N}. \\ \text{(d) } x \in [-1,1]. \\ 2.33 \\ \text{(a) } P(1,-1): \text{false}; P(3,4): \text{false}; P(5,5): \text{true}. \\ \text{(b) }P(1,2): \text{true}; P(2,-2): \text{false}; P(6,6): \text{true}. \\ \text{(c) } P(1,-1): \text{true}; P(-3,4): \text{true}; P(0,-1): \text{true}; P(1,0): \text{true}. \\ 2.34 \\ \text{(a) If any point on the straight line with equation } 2y + x - 3 = 0 \text{ where x-coordinate is an integer, then y-coordinate is also an integer.} \\ \text{(b) If the integer odd, then the square of that of integer is odd.} \\ \text{(c) If any integer n satisfies } 3n + 7 \text{ is even, then n is odd.} \\ \text{(d) If the function } f(x) = cosx, \text{ then the derivative of the function } f(x) \text{ is } f'(x) = sinx. \\ \text{(e) If } C \text{ is the circle of circumference } 4\pi \text{, then the area of } C \text{ is } 4\pi. \\ \text{(f) If the integer } n \text{ is even, then the integer } n^3 \text{ is even.} \\ 2.35 \\ \text{18 is odd if and only if 25 is even.} - \text{ This statement is true.} \\ 2.36 \\ (1) \text{ The integer } n \text{ is odd if and only if } n^2 \text{ is odd.} \\ (2) \text{ The integer } n \text{ is odd and } n^2 \text{ is odd are jointly necessary and sufficient for one another.} \\ 2.37 \\ 1) |x - 3| < 1 \text{ is equivalent to } x \in (2,4). \\ 2) |x - 3| < 1 \text{ if and only if } x \in (2,4). \\ 2.38 \\ \text{(a) "} x \text{ is not equal to } -2 \text{" is true for } x = 0 \vee x = 2. \\ \text{(b) "} \text{Either } x = -2 \text{ or } x^2 = 4 \text{" is true for } x = -2 \vee x = 2. \\ \text{(c) "Both } x = -2 \text{ and  } x^2 = 4 \text{" is true for } x = 2. \\ \text{(d) "If } x = -2 \text{ then } x^2 = 4 \text{" is true for every } x \in S. \\ \text{(e) "If } x^2 = 4 \text{ then } x = -2 \text{" is true for every } x \in S. \\ \text{(f) "} x = -2 \text{ if and only if } x^2 = 4 \text{" is true for } x = -2. \\ 2.39 \\ \text{(a) } x = 4. \\ \text{(b) } x \in \{4,6\}. \\ \text{(c) } x = 4. \\ 2.40 \\ \text{(a) } P(1,-1) \wedge Q(1,-1) \text{ is false.} \\ P(3,4) \wedge Q(3,4) \text{ is false.} \\ P(5,5) \wedge Q(5,5) \text{ is true.} \\ \text{(b) } P(1,2) \wedge Q(1,2) \text{ is false.} \\ P(2,-2) \wedge Q(2,-2) \text{ is false.} \\ P(6,6) \wedge Q(6,6) \text{ is true.} \\ \text{(c) } P(1,-1) \wedge Q(1,-1) \text{ is false.} \\ P(-3,4) \wedge Q(-3,4) \text{ is false.} \\ P(0,-1) \wedge Q(0,-1) \text{ is true.} \\ P(1,0) \wedge Q(1,0) \text{ is true.} \\ 2.41 \\ n = 3. \\ 2.42 \\ n = 3. \\ 2.43 \\ a = 1; b = 3; c = 2. \\ 2.44 \\ (i) a = 1. \\ (ii) b = 1 \vee b = 4. \\ (iii) c = 1 \vee c = 2 \vee c = 3. \\ (iv) d = 2 \vee d = 3 \vee d = 4. \\ 2.45 \\ n \in \{2,3,5\}. \\ 2.46 \\
\begin{array}{|c|c|c|c|}
   \hline
   P & Q & P \vee Q & P \Rightarrow (P \vee Q) \\ 
   \hline
   T & T & T & T\\
   \hline
   T & F & T & T\\
   \hline
   F & T & T & T\\
   \hline
   F & F & F & T\\
   \hline
\end{array} \\ 
\text{We can conclude that  } P \Rightarrow (P \vee Q) \text{ is a tautology.} \\ 2.47 \\ \begin{array} {|c|c|c|c|c|c|c|c|}
   \hline
   P & Q & \sim Q & P \wedge (\sim Q) & P \wedge Q & P \Rightarrow \sim Q & (P \wedge (\sim Q)) \wedge (P \wedge Q) & (P \Rightarrow (\sim Q)) \wedge (P \wedge Q) \\ \hline
   T & T & F & F & T & F & F & F\\
   \hline
   T & F & T & T & F & T & F & F\\
   \hline
   F & T & F & T & F & T & F & F\\
   \hline
   F & F & T & T & F & T & F & F\\
   \hline
\end{array} \\ \text{We can conclude that } (P \wedge (\sim Q)) \wedge (P \wedge Q) \text{ and } (P \Rightarrow (\sim Q)) \wedge (P \wedge Q) \text{ are both contradictions.} \\ 2.48 \\ \begin{array} {|c|c|c|c|}
   \hline
   P & Q & P \Rightarrow Q & (P \wedge (P \Rightarrow Q)) \Rightarrow Q \\
   \hline
   T & T & T & T\\
   \hline
   T & F & F & T\\
   \hline
   F & T & T & T\\
   \hline
   F & F & T & T\\
   \hline
\end{array} \\ \text{Base on the truth table, } (P \wedge (P \Rightarrow Q)) \Rightarrow Q \text{ is a tautology.} \\ "(P \wedge (P \Rightarrow Q)) \Rightarrow Q": \text{If } P \text{ and } P \text{ implies } Q, \text{ then Q.} \\ 2.49 \\ \begin{array} {|c|c|c|c|c|c|c|}
\hline
   P & Q & R & P \Rightarrow Q & Q \Rightarrow R & P \Rightarrow R & ((P \Rightarrow Q) \wedge (Q \Rightarrow R) \Rightarrow (P \Rightarrow R))\\
   \hline
   T & T & T & T & T & T & T\\
   \hline
   T & F & F & F & T & F & T\\
   \hline
   F & T & F & T & F & T & T\\
   \hline
   F & F & T & T & T & T & T\\
   \hline
\end{array} \\ \text{We can conclude that } ((P \Rightarrow Q) \wedge (Q \Rightarrow R) \Rightarrow (P \Rightarrow R)) \text{ is a tautology.} \\ "((P \Rightarrow Q) \wedge (Q \Rightarrow R) \Rightarrow (P \Rightarrow R))": \text{If } P \text{ implies } Q \text{ and } Q \text{ implies } R, \text{ then } P \text{ implies } R. \\}$ 
$\Large{ 2.50 \\ \Large\text{For } R \text{ is a tautology, } S \text{ is a contradiction, we have the following corrolaries:} \\ \text{(a) This statement is always true.} \\ \text{(b) This statement is always false.} \\ \text{(c) This statement is always false.} \\ \text{(d) This statement is always true.} \\}$ 
$\Large{2.51 \\ \begin{array} {|c|c|c|c|c|}
   \hline
   P & Q & P \vee Q & Q \Rightarrow P & (P \vee Q) \vee (Q \Rightarrow P)\\
   \hline
   T & T & T & T & T\\
   \hline
   T & F & T & T & T\\
   \hline
   F & T & T & F & T\\
   \hline
   F & F & F & T & T\\
   \hline
\end{array} \\ \text{We can conclude that } (P \vee Q) \vee (Q \Rightarrow P) \text{ is a tautology.} \\ 2.52 \\ \Large\begin{array} {|c|c|c|c|c|}
\hline
P & Q & P \Rightarrow Q & Q \Rightarrow P & ((P \Rightarrow Q) \Rightarrow P) \Rightarrow (P \Rightarrow (Q \Rightarrow P))\\
\hline
T & T & T & T & T\\
\hline
T & F & F & T & T\\
\hline
F & T & T & F & T\\
\hline
F & F & T & T & T\\
\hline	
\end{array} \\ \text{We can conclude that } ((P \Rightarrow Q) \Rightarrow P) \Rightarrow (P \Rightarrow (Q \Rightarrow P)) \text{ is a tautology.} \\ 2.53 \\ \text{(a) } \\ \begin{array} {|c|c|c|c|c|c|} 
\hline
P & Q & \sim P & \sim Q & P \Rightarrow Q & (\sim P) \Rightarrow (\sim Q)\\
\hline
T & T & F & F & T & T\\
\hline
T & F & F & T & F & T\\
\hline
F & T & T & T & T & T\\
\hline
F & F & T & F & T & F\\
\hline
\end{array} \\ \text{(b) } (\sim P) \Rightarrow (\sim Q) \text{ is logically equivalent to } P \vee Q. \\ \begin{array} {|c|c|c|c|c|c|} 
\hline
P & Q & \sim P & \sim Q & P \vee Q & (\sim P) \Rightarrow (\sim Q)\\
\hline
T & T & F & F & T & T\\
\hline
T & F & F & T & T & T\\
\hline
F & T & T & T & T & T\\
\hline
F & F & T & F & F & F\\
\hline
\end{array} \\ 2.54 \\ \text{(a) } \\ \begin{array} {|c|c|c|c|c|c|} 
\hline
P & Q & \sim P & \sim Q & \sim(P \vee Q) & (\sim P) \vee (\sim Q)\\
\hline
T & T & F & F & F & F\\
\hline
T & F & F & T & F & T\\
\hline
F & T & T & F & F & T\\
\hline
F & F & T & T & T & T\\
\hline
\end{array} \\ \text{Since, } \sim(P \vee Q) \text{ do not have the same truth values for all combinations of truth values for the component statements } P \text{ and } Q, \sim(P \vee Q) \text{ is not logically equivalent to } (\sim P) \vee (\sim Q). \\ \text{(b) The biconditional } \sim(P \vee Q) \text{ and } (\sim P) \vee (\sim Q) \text{ is not a tautology since not all combinations of truth values from two statements are the same.} \\ 2.55 \\ \text{(a) } \\ \begin{array} {|c|c|c|c|} 
\hline
P & Q & (P \wedge Q) \Leftrightarrow P & P \Rightarrow Q\\
\hline
T & T & T & T\\
\hline
T & F & F & F\\
\hline
F & T & T & T\\
\hline
F & F & T & T\\
\hline
\end{array} \\ \text{(b) } \\ \begin{array} {|c|c|c|c|c|c|c|} 
\hline
P & Q & R & \sim P & \sim Q & P \Rightarrow (Q \vee R) & (\sim Q) \Rightarrow ((\sim P) \vee R)\\
\hline
T & T & F & F & F & T & T\\
\hline
T & F & T & F & T & T & T\\
\hline
F & T & F & T & F & T & T\\
\hline
F & F & T & T & T & T & T\\
\hline
\end{array} \\ 2.56 \\ (\sim Q) \Rightarrow (P \vee (\sim P)) \text{ and } Q \text{ are logically equivalent since they have the same truth values for all combinations of truth values for the component statements P and Q.} \\ \begin{array} {|c|c|c|c|c|} 
\hline
P & Q & \sim P & \sim Q & (\sim Q) \Rightarrow (P \wedge (\sim P))\\
\hline
T & T & F & F & T\\
\hline
T & F & F & T & F\\
\hline
F & T & T & F & T\\
\hline
F & F & T & T & F\\
\hline
\end{array} \\ 2.57 \\ (P \vee Q) \Rightarrow R \text{ and } (P \Rightarrow R) \wedge (Q \Rightarrow R) \text{ are logically equivalent since they have the same truth values for all combinations of truth values for the component statements } P, Q \text{ and } R. \\ \begin{array} {|c|c|c|c|c|} 
\hline
P & Q & R & (P \vee Q) \Rightarrow R & (P \Rightarrow R) \wedge (Q \Rightarrow R)\\
\hline
T & T & F & F & F\\
\hline
T & F & T & T & F\\
\hline
F & T & F & F & F\\
\hline
F & F & T & T & T\\
\hline
\end{array} \\ 2.58 \\ \text{If } S \text{ and } T \text{ are not logically equivalent, then there is some combinations of truth values of the component statements } P, Q \text{ and } R \text{ for which } S \text{ and } T \text{ have different truth values.} \\ 2.59 \\ \text{Since there are only four different combinations of truth values of } P \text{ and } Q \text{ for the second and third row of the statements } S_1, S_2, S_3, S_4 \text{ and } S_5, \text{ at least two of these statements must have identical truth tables and so are logically equivalent.} \\ 2.60 \\ \text{(a) } P \vee (Q \wedge R) \text{ and } (P \vee Q) \wedge (P \vee R) \text{ are logically equivalent since they have the same truth values in Figure 2.19.} \\ \text{(b) } \sim (P \vee Q) \text{ and } (\sim P) \wedge (\sim Q) \text{are logically equivalent since they have the same truth values according to De Morgan's Laws.} \\ 2.61 \\ \text{(a) Both } x \neq 0 \text{ and } y \neq 0. \\ \text{(b) Either the integer } a \text{ is odd or the integer } b \text{ is odd.} \\ 2.62 \\ \text{(a) } xy \text{ is even only if } x \text{ and } y \text{ are even.} \\ \text{(b) If either } x \text{ or } y \text{ is odd, then } xy \text{ is odd.} \\ \text{(c) At least one of } x \text{ and } y \text{ are even or } xy \text{ is even.} \\ \text{(d) } x \text{ and } y \text{ are even and } xy \text{ is even.} \\ 2.63 \\ \text{Either } x^2 = 2 \text{ and } x \neq \sqrt{2} \text{ or } x = \sqrt{2} \text{ and } x^2 \neq 2. \\ 2.64 \\ \begin{array} {cccr} 
[P \vee Q \wedge (\sim(P \wedge Q))] & = & [(P \vee Q) \vee ((\sim P) \wedge (\sim Q))]\\
& = & (P \wedge (\sim P)) \vee (P \wedge (\sim Q)) \vee (Q \wedge (\sim P)) \vee (Q \wedge (\sim Q))\\
& = & \sim(P \Leftrightarrow Q) & \blacksquare\\
\end{array} \\ 2.65 \\ \text{If the integer } 3n+4 \text{ is odd, then } 5n-6 \text{ is odd.} \\ 2.66 \\ n^3 \text{ is odd if and only if } 7n+2 \text{ is even.}}$

$\\ \Large \text{[N]: There are some alternative ways to express } P \Leftrightarrow Q \text{ in words}: \\ \large -\text{ A necessary and sufficient condition for P is (that) Q.} \\ \large -P \text{ and } Q \text{ are jointly necessary and sufficient for one another.}$